OCamlに変換する関数書いた＆同値を証明

typeArith/ocaml/src/eval.ml
@@ -1,0 +1,125 @@
+
+type bool =
+| True
+| False
+
+type term =
+| Tru
+| Fls
+| If of term * term * term
+| O
+| Succ of term
+| Pred of term
+| Iszero of term
+
+(** val natValue : term -> bool **)
+
+let rec natValue = function
+| O -> True
+| Succ t1 -> natValue t1
+| _ -> False
+
+(** val value : term -> bool **)
+
+let rec value t0 = match t0 with
+| Tru -> True
+| Fls -> True
+| _ -> natValue t0
+
+type t =
+| Bool
+| Nat
+
+type optionT =
+| SomeT of t
+| NoneT
+
+(** val eqT : t -> t -> bool **)
+
+let eqT t1 t2 =
+  match t1 with
+  | Bool -> (match t2 with
+             | Bool -> True
+             | Nat -> False)
+  | Nat -> (match t2 with
+            | Bool -> False
+            | Nat -> True)
+
+(** val has_type : term -> optionT **)
+
+let rec has_type = function
+| If (t1, t2, t3) ->
+  (match has_type t1 with
+   | SomeT t4 ->
+     (match t4 with
+      | Bool ->
+        (match has_type t2 with
+         | SomeT t5 ->
+           (match has_type t3 with
+            | SomeT t6 -> (match eqT t5 t6 with
+                           | True -> SomeT t5
+                           | False -> NoneT)
+            | NoneT -> NoneT)
+         | NoneT -> NoneT)
+      | Nat -> NoneT)
+   | NoneT -> NoneT)
+| O -> SomeT Nat
+| Succ t1 -> (match has_type t1 with
+              | SomeT t2 -> (match t2 with
+                             | Bool -> NoneT
+                             | Nat -> SomeT Nat)
+              | NoneT -> NoneT)
+| Pred t1 -> (match has_type t1 with
+              | SomeT t2 -> (match t2 with
+                             | Bool -> NoneT
+                             | Nat -> SomeT Nat)
+              | NoneT -> NoneT)
+| Iszero t1 ->
+  (match has_type t1 with
+   | SomeT t2 -> (match t2 with
+                  | Bool -> NoneT
+                  | Nat -> SomeT Bool)
+   | NoneT -> NoneT)
+| _ -> SomeT Bool
+
+type optiont =
+| Some of term
+| None
+
+(** val eval : term -> optiont **)
+
+let rec eval = function
+| If (t1, t2, t3) ->
+  (match value t1 with
+   | True -> (match t1 with
+              | Tru -> Some t2
+              | Fls -> Some t3
+              | _ -> None)
+   | False -> (match eval t1 with
+               | Some t1' -> Some (If (t1', t2, t3))
+               | None -> None))
+| Succ t1 ->
+  (match natValue t1 with
+   | True -> None
+   | False -> (match eval t1 with
+               | Some t1' -> Some (Succ t1')
+               | None -> None))
+| Pred t1 ->
+  (match natValue t1 with
+   | True -> (match t1 with
+              | O -> Some O
+              | Succ nv1 -> Some nv1
+              | _ -> None)
+   | False -> (match eval t1 with
+               | Some t1' -> Some (Pred t1')
+               | None -> None))
+| Iszero t1 ->
+  (match natValue t1 with
+   | True -> (match t1 with
+              | O -> Some Tru
+              | Succ _ -> Some Fls
+              | _ -> None)
+   | False -> (match eval t1 with
+               | Some t1' -> Some (Iszero t1')
+               | None -> None))
+| _ -> None
