typeArith/ocaml/src/eval.mli
@@ -1,0 +1,35 @@
+
+type bool =
+| True
+| False
+
+type term =
+| Tru
+| Fls
+| If of term * term * term
+| O
+| Succ of term
+| Pred of term
+| Iszero of term
+
+val natValue : term -> bool
+
+val value : term -> bool
+
+type t =
+| Bool
+| Nat
+
+type optionT =
+| SomeT of t
+| NoneT
+
+val eqT : t -> t -> bool
+
+val has_type : term -> optionT
+
+type optiont =
+| Some of term
+| None
+
+val eval : term -> optiont
